Foundation/IntProp/Hilbert2/Basic.lean
@@ -1,0 +1,273 @@
+import Foundation.Logic.HilbertStyle.Supplemental
+import Foundation.IntProp.Formula
+
+namespace LO.IntProp
+
+variable {α : Type u}
+
+structure Hilbert (α) where
+  axioms : Set (Formula α)
+
+class Hilbert.FiniteAxiomatizable (H : Hilbert α) where
+  axioms_fin : Set.Finite H.axioms
+
+class Hilbert.HasEFQ (H : Hilbert α) where
+  p : α
+  mem_efq : (⊥ ➝ (.atom p)) ∈ H.axioms := by tauto;
+
+class Hilbert.HasLEM (H : Hilbert α) where
+  p : α
+  mem_lem : (.atom p ⋎ ∼(.atom p)) ∈ H.axioms := by tauto;
+
+class Hilbert.HasDNE (H : Hilbert α) where
+  p : α
+  mem_dne : (∼∼(.atom p) ➝ (.atom p)) ∈ H.axioms := by tauto;
+
+class Hilbert.HasWeakLEM (H : Hilbert α) where
+  p : α
+  mem_wlem : (∼(.atom p) ⋎ ∼∼(.atom p)) ∈ H.axioms := by tauto;
+
+class Hilbert.HasDummett (H : Hilbert α) where
+  p : α
+  q : α
+  ne_pq : p ≠ q
+  mem_dummet : ((.atom p) ➝ (.atom q)) ⋎ ((.atom q) ➝ (.atom p)) ∈ H.axioms := by tauto;
+
+namespace Hilbert
+
+variable {H : Hilbert α}
+
+inductive Deduction (H : Hilbert α) : Formula α → Type _
+  | eaxm {φ}      : φ ∈ H.axioms → Deduction H φ
+  | mdp {φ ψ}     : Deduction H (φ ➝ ψ) → Deduction H φ → Deduction H ψ
+  | subst {φ} (s) : Deduction H φ → Deduction H (φ⟦s⟧)
+  | verum         : Deduction H $ ⊤
+  | implyS φ ψ    : Deduction H $ φ ➝ ψ ➝ φ
+  | implyK φ ψ χ  : Deduction H $ (φ ➝ ψ ➝ χ) ➝ (φ ➝ ψ) ➝ φ ➝ χ
+  | andElimL φ ψ  : Deduction H $ φ ⋏ ψ ➝ φ
+  | andElimR φ ψ  : Deduction H $ φ ⋏ ψ ➝ ψ
+  | andIntro φ ψ  : Deduction H $ φ ➝ ψ ➝ φ ⋏ ψ
+  | orIntroL φ ψ  : Deduction H $ φ ➝ φ ⋎ ψ
+  | orIntroR φ ψ  : Deduction H $ ψ ➝ φ ⋎ ψ
+  | orElim φ ψ χ  : Deduction H $ (φ ➝ χ) ➝ (ψ ➝ χ) ➝ (φ ⋎ ψ ➝ χ)
+
+instance : System (Formula α) (Hilbert α) := ⟨Deduction⟩
+
+open Deduction
+open Hilbert
+
+section
+
+instance : System.ModusPonens H := ⟨mdp⟩
+
+instance : System.HasAxiomImply₁ H := ⟨implyS⟩
+
+instance : System.HasAxiomImply₂ H := ⟨implyK⟩
+
+instance : System.HasAxiomAndInst H := ⟨andIntro⟩
+
+instance : System.Minimal H where
+  mdp := mdp
+  verum := verum
+  and₁ := andElimL
+  and₂ := andElimR
+  and₃ := andIntro
+  or₁ := orIntroL
+  or₂ := orIntroR
+  or₃ := orElim
+
+section
+
+variable [DecidableEq α]
+
+instance [efq : H.HasEFQ] : System.HasAxiomEFQ H where
+  efq φ := by simpa using subst (s := λ b => if b = efq.p then φ else (.atom b)) $ eaxm efq.mem_efq;
+
+instance [lem : H.HasLEM]  : System.HasAxiomLEM H where
+  lem φ := by simpa using subst (s := λ b => if b = lem.p then φ else (.atom b)) $ eaxm lem.mem_lem;
+
+instance [dne : H.HasDNE] : System.HasAxiomDNE H where
+  dne φ := by simpa using subst (s := λ b => if b = dne.p then φ else (.atom b)) $ eaxm dne.mem_dne;
+
+instance [wlem : H.HasWeakLEM] : System.HasAxiomWeakLEM H where
+  wlem φ := by simpa using subst (s := λ b => if b = wlem.p then φ else (.atom b)) $ eaxm wlem.mem_wlem;
+
+instance [dummet : H.HasDummett] : System.HasAxiomDummett H where
+  dummett φ ψ := by
+    simpa [dummet.ne_pq, bne_iff_ne, ne_eq] using
+      subst
+        (s := λ b =>
+          if dummet.p = b then φ
+          else if dummet.q = b then ψ
+          else (.atom b)
+        )
+        $ eaxm dummet.mem_dummet;
+
+instance [H.HasEFQ] : System.Intuitionistic H where
+
+instance [H.HasDNE] : System.Classical H where
+
+end
+
+end
+
+
+abbrev theorems (H : Hilbert α) : Set (Formula α) := System.theory H
+
+
+section systems
+
+variable (α) [DecidableEq α]
+
+protected abbrev Minimal : Hilbert α := ⟨∅⟩
+
+section
+
+variable [hα : HasElements 1 α]
+
+protected abbrev Int : Hilbert α := ⟨{⊥ ➝ (.atom (hα.fn 0))}⟩
+
+instance : (Hilbert.Int α).HasEFQ where p := (hα.fn 0)
+
+instance : System.Intuitionistic (Hilbert.Int α) where
+
+instance : (Hilbert.Int α).FiniteAxiomatizable where axioms_fin := by simp
+
+end
+
+
+
+section
+
+variable [hα : HasElements 1 α]
+
+protected abbrev Cl : Hilbert α := ⟨{⊥ ➝ (.atom (hα.fn 0)), (.atom (hα.fn 0) ⋎ ∼(.atom (hα.fn 0)))}⟩
+instance : (Hilbert.Cl α).HasLEM where p := (hα.fn 0);
+instance : (Hilbert.Cl α).HasEFQ where p := (hα.fn 0);
+
+end
+
+
+section
+
+variable [hα : HasElements 1 α]
+
+/--
+  `KC` from Chagrov & Zakharyaschev (1997)
+-/
+protected abbrev KC : Hilbert α := ⟨{⊥ ➝ (.atom (hα.fn 0)), ∼(.atom (hα.fn 0)) ⋎ ∼∼(.atom (hα.fn 0))}⟩
+instance : (Hilbert.KC α).HasEFQ where p := (hα.fn 0)
+instance : (Hilbert.KC α).HasWeakLEM where p := (hα.fn 0)
+
+end
+
+
+section
+
+variable [hα : HasElements 2 α]
+
+/--
+  `LC` from Chagrov & Zakharyaschev (1997)
+-/
+protected abbrev LC : Hilbert α := ⟨{⊥ ➝ (.atom (hα.fn 0)), ((.atom (hα.map 0) ➝ .atom (hα.map 1)) ⋎ (.atom (hα.map 1) ➝ .atom (hα.map 0)))}⟩
+instance : (Hilbert.LC α).HasEFQ where p := (hα.fn 0)
+instance : (Hilbert.LC α).HasDummett where
+  p := (hα.fn 0);
+  q := (hα.fn 1);
+  ne_pq := hα.distinct (by trivial)
+
+end
+
+end systems
+
+
+abbrev Consistent (H : Hilbert α) := System.Consistent H
+
+
+namespace Deduction
+
+open System
+
+variable {H : Hilbert α} {φ ψ : Formula α}
+
+lemma eaxm! (h : φ ∈ H.axioms) : H ⊢! φ := ⟨eaxm h⟩
+
+lemma mdp! (hpq : H ⊢! (φ ➝ ψ)) (hp : H ⊢! φ) : H ⊢! ψ := ⟨mdp hpq.some hp.some⟩
+
+lemma subst! (hp : H ⊢! φ) (s : Substitution α) : H ⊢! (φ⟦s⟧) := ⟨subst s hp.some⟩
+
+noncomputable def rec! {α : Type u} {H : Hilbert α}
+  {motive : (a : Formula α) → H ⊢! a → Sort u_1}
+  (hAxm   : ∀ {φ}, (a : φ ∈ H.axioms) → motive φ ⟨eaxm a⟩)
+  (hMdp    : ∀ {φ ψ}, {hpq : H ⊢! (φ ➝ ψ)} → {hp : H ⊢! φ} → motive (φ ➝ ψ) hpq → motive φ hp → motive ψ (mdp! hpq hp))
+  (hSubst  : ∀ {φ s}, {hp : H ⊢! φ} → motive φ hp → motive (φ⟦s⟧) (subst! hp s))
+  (hVerum  : motive ⊤ verum!)
+  (hImply₁ : ∀ {φ ψ},   motive (φ ➝ ψ ➝ φ) imply₁!)
+  (hImply₂ : ∀ {φ ψ χ}, motive ((φ ➝ ψ ➝ χ) ➝ (φ ➝ ψ) ➝ φ ➝ χ) imply₂!)
+  (hAnd₁   : ∀ {φ ψ},   motive (φ ⋏ ψ ➝ φ) and₁!)
+  (hAnd₂   : ∀ {φ ψ},   motive (φ ⋏ ψ ➝ ψ) and₂!)
+  (hAnd₃   : ∀ {φ ψ},   motive (φ ➝ ψ ➝ φ ⋏ ψ) and₃!)
+  (hOr₁    : ∀ {φ ψ},   motive (φ ➝ φ ⋎ ψ) or₁!)
+  (hOr₂    : ∀ {φ ψ},   motive (ψ ➝ φ ⋎ ψ) or₂!)
+  (hOr₃    : ∀ {φ ψ χ}, motive ((φ ➝ χ) ➝ (ψ ➝ χ) ➝ φ ⋎ ψ ➝ χ) or₃!) :
+  {a : Formula α} → (t : H ⊢! a) → motive a t := by
+  intro φ d;
+  induction d.some with
+  | eaxm h => exact hAxm h
+  | mdp hpq hp ihpq ihp => exact hMdp (ihpq ⟨hpq⟩) (ihp ⟨hp⟩)
+  | subst s hp ihp => exact hSubst (ihp ⟨hp⟩);
+  | _ => aesop
+
+end Deduction
+
+
+open System
+
+section
+
+lemma weaker_than_of_subset_axiomset' {H₁ H₂ : Hilbert α} (hMaxm : ∀ {φ : Formula α}, φ ∈ H₁.axioms → H₂ ⊢! φ)
+  : H₁ ≤ₛ H₂ := by
+  apply System.weakerThan_iff.mpr;
+  intro φ h;
+  induction h using Deduction.rec! with
+  | hAxm hp => apply hMaxm hp;
+  | hMdp ihpq ihp => exact ihpq ⨀ ihp;
+  | hSubst hp => exact subst! hp _;
+  | _ => simp;
+
+lemma weaker_than_of_subset_axiomset {H₁ H₂ : Hilbert α} (hSubset : H₁.axioms ⊆ H₂.axioms := by aesop) : H₁ ≤ₛ H₂ := by
+  apply weaker_than_of_subset_axiomset';
+  intro φ hp;
+  apply eaxm! $ hSubset hp;
+
+lemma Int_weaker_than_Cl [HasElements 1 α]: (Hilbert.Int α) ≤ₛ (Hilbert.Cl α) := weaker_than_of_subset_axiomset
+
+lemma Int_weaker_than_KC [HasElements 1 α] : (Hilbert.Int α) ≤ₛ (Hilbert.KC α) := weaker_than_of_subset_axiomset
+
+/-
+lemma Int_weaker_than_LC [HasElements 1 α] [HasElements 2 α] : (Hilbert.Int α) ≤ₛ (Hilbert.LC α) := weaker_than_of_subset_axiomset
+
+lemma KC_weaker_than_Cl [HasElements 1 α] : (Hilbert.KC α) ≤ₛ (Hilbert.Cl α) := weaker_than_of_subset_axiomset' $ by
+  rintro φ (⟨_, rfl⟩ | ⟨_, rfl⟩);
+  . sorry;
+  . sorry;
+
+lemma LC_weaker_than_Cl [DecidableEq α] [HasElements 2 α] : (Hilbert.LC α) ≤ₛ (Hilbert.Cl α) := by
+  apply weaker_than_of_subset_axiomset';
+  rintro φ (⟨_, rfl⟩ | ⟨_, _, rfl⟩);
+  . sorry;
+  . sorry;
+
+lemma KC_weaker_than_LC [DecidableEq α] [HasElements 2 α] : (Hilbert.KC α) ≤ₛ (Hilbert.LC α) := by
+  apply weaker_than_of_subset_axiomset';
+  rintro φ (⟨_, rfl⟩ | ⟨_, rfl⟩)
+  . sorry;
+  . sorry;
+-/
+
+end
+
+
+end Hilbert
+
+end LO.IntProp
